Regenerate sandwich-api-proto dependencies.

proofs/fstar/extraction/Sandwich.Error.Code.fsti
@@ -9,287 +9,316 @@ let _ =
   let open Sandwich_proto.Errors in
   ()
 
+/// An enum allowed in [`ProtoBasedErrorCode`].
+class t_AllowedProtoBasedErrorCodeEnum (v_Self: Type0) = {
+  [@@@ FStar.Tactics.Typeclasses.no_method]_super_11581440318597584651:Core.Marker.t_Copy v_Self;
+  [@@@ FStar.Tactics.Typeclasses.no_method]_super_9442900250278684536:Core.Clone.t_Clone v_Self
+}
+
+/// Adds `ErrorEnum` to the list of [`AllowedProtoBasedErrorCodeEnum`] trait.
+[@@ FStar.Tactics.Typeclasses.tcinstance]
+val impl_77:t_AllowedProtoBasedErrorCodeEnum Sandwich_proto.Errors.t_ALPNError
+
+[@@ FStar.Tactics.Typeclasses.tcinstance]
+val impl_78:t_AllowedProtoBasedErrorCodeEnum Sandwich_proto.Errors.t_ALPNError
+
+/// Adds `ErrorEnum` to the list of [`AllowedProtoBasedErrorCodeEnum`] trait.
+[@@ FStar.Tactics.Typeclasses.tcinstance]
+val impl_14:t_AllowedProtoBasedErrorCodeEnum Sandwich_proto.Errors.t_APIError
+
+[@@ FStar.Tactics.Typeclasses.tcinstance]
+val impl_15:t_AllowedProtoBasedErrorCodeEnum Sandwich_proto.Errors.t_APIError
+
+/// Adds `ErrorEnum` to the list of [`AllowedProtoBasedErrorCodeEnum`] trait.
+[@@ FStar.Tactics.Typeclasses.tcinstance]
+val impl_68:t_AllowedProtoBasedErrorCodeEnum Sandwich_proto.Errors.t_ASN1Error
+
+[@@ FStar.Tactics.Typeclasses.tcinstance]
+val impl_69:t_AllowedProtoBasedErrorCodeEnum Sandwich_proto.Errors.t_ASN1Error
+
+/// Adds `ErrorEnum` to the list of [`AllowedProtoBasedErrorCodeEnum`] trait.
+[@@ FStar.Tactics.Typeclasses.tcinstance]
+val impl_50:t_AllowedProtoBasedErrorCodeEnum Sandwich_proto.Errors.t_CertificateError
+
+[@@ FStar.Tactics.Typeclasses.tcinstance]
+val impl_51:t_AllowedProtoBasedErrorCodeEnum Sandwich_proto.Errors.t_CertificateError
+
+/// Adds `ErrorEnum` to the list of [`AllowedProtoBasedErrorCodeEnum`] trait.
+[@@ FStar.Tactics.Typeclasses.tcinstance]
+val impl_23:t_AllowedProtoBasedErrorCodeEnum Sandwich_proto.Errors.t_ConfigurationError
+
+[@@ FStar.Tactics.Typeclasses.tcinstance]
+val impl_24:t_AllowedProtoBasedErrorCodeEnum Sandwich_proto.Errors.t_ConfigurationError
+
+/// Adds `ErrorEnum` to the list of [`AllowedProtoBasedErrorCodeEnum`] trait.
+[@@ FStar.Tactics.Typeclasses.tcinstance]
+val impl_86:t_AllowedProtoBasedErrorCodeEnum Sandwich_proto.Errors.t_DataSourceError
+
+[@@ FStar.Tactics.Typeclasses.tcinstance]
+val impl_87:t_AllowedProtoBasedErrorCodeEnum Sandwich_proto.Errors.t_DataSourceError
+
+/// Adds `ErrorEnum` to the list of [`AllowedProtoBasedErrorCodeEnum`] trait.
+[@@ FStar.Tactics.Typeclasses.tcinstance]
+val impl_122:t_AllowedProtoBasedErrorCodeEnum Sandwich_proto.Errors.t_HandshakeError
+
+[@@ FStar.Tactics.Typeclasses.tcinstance]
+val impl_123:t_AllowedProtoBasedErrorCodeEnum Sandwich_proto.Errors.t_HandshakeError
+
+/// Adds `ErrorEnum` to the list of [`AllowedProtoBasedErrorCodeEnum`] trait.
+[@@ FStar.Tactics.Typeclasses.tcinstance]
+val impl_95:t_AllowedProtoBasedErrorCodeEnum Sandwich_proto.Errors.t_KEMError
+
+[@@ FStar.Tactics.Typeclasses.tcinstance]
+val impl_96:t_AllowedProtoBasedErrorCodeEnum Sandwich_proto.Errors.t_KEMError
+
+/// Adds `ErrorEnum` to the list of [`AllowedProtoBasedErrorCodeEnum`] trait.
+[@@ FStar.Tactics.Typeclasses.tcinstance]
+val impl_59:t_AllowedProtoBasedErrorCodeEnum Sandwich_proto.Errors.t_PrivateKeyError
+
+[@@ FStar.Tactics.Typeclasses.tcinstance]
+val impl_60:t_AllowedProtoBasedErrorCodeEnum Sandwich_proto.Errors.t_PrivateKeyError
+
+/// Adds `ErrorEnum` to the list of [`AllowedProtoBasedErrorCodeEnum`] trait.
+[@@ FStar.Tactics.Typeclasses.tcinstance]
+val impl_32:t_AllowedProtoBasedErrorCodeEnum Sandwich_proto.Errors.t_ProtobufError
+
+[@@ FStar.Tactics.Typeclasses.tcinstance]
+val impl_33:t_AllowedProtoBasedErrorCodeEnum Sandwich_proto.Errors.t_ProtobufError
+
+/// Adds `ErrorEnum` to the list of [`AllowedProtoBasedErrorCodeEnum`] trait.
+[@@ FStar.Tactics.Typeclasses.tcinstance]
+val impl_113:t_AllowedProtoBasedErrorCodeEnum Sandwich_proto.Errors.t_SocketError
+
+[@@ FStar.Tactics.Typeclasses.tcinstance]
+val impl_114:t_AllowedProtoBasedErrorCodeEnum Sandwich_proto.Errors.t_SocketError
+
+/// Adds `ErrorEnum` to the list of [`AllowedProtoBasedErrorCodeEnum`] trait.
+[@@ FStar.Tactics.Typeclasses.tcinstance]
+val impl_104:t_AllowedProtoBasedErrorCodeEnum Sandwich_proto.Errors.t_SystemError
+
+[@@ FStar.Tactics.Typeclasses.tcinstance]
+val impl_105:t_AllowedProtoBasedErrorCodeEnum Sandwich_proto.Errors.t_SystemError
+
+/// Adds `ErrorEnum` to the list of [`AllowedProtoBasedErrorCodeEnum`] trait.
+[@@ FStar.Tactics.Typeclasses.tcinstance]
+val impl_41:t_AllowedProtoBasedErrorCodeEnum Sandwich_proto.Errors.t_TLSConfigurationError
+
+[@@ FStar.Tactics.Typeclasses.tcinstance]
+val impl_42:t_AllowedProtoBasedErrorCodeEnum Sandwich_proto.Errors.t_TLSConfigurationError
+
+/// Adds `ErrorEnum` to the list of [`AllowedProtoBasedErrorCodeEnum`] trait.
+[@@ FStar.Tactics.Typeclasses.tcinstance]
+val impl_131:t_AllowedProtoBasedErrorCodeEnum Sandwich_proto.Errors.t_TunnelError
+
+[@@ FStar.Tactics.Typeclasses.tcinstance]
+val impl_132:t_AllowedProtoBasedErrorCodeEnum Sandwich_proto.Errors.t_TunnelError
+
+/// An error code.
+/// An error code holds one of the error described in `errors.proto`
+/// and listed in `ErrorKind`.
+type t_ProtoBasedErrorCode =
+  | ProtoBasedErrorCode_APIError : Sandwich_proto.Errors.t_APIError -> t_ProtoBasedErrorCode
+  | ProtoBasedErrorCode_ConfigurationError : Sandwich_proto.Errors.t_ConfigurationError
+    -> t_ProtoBasedErrorCode
+  | ProtoBasedErrorCode_ProtobufError : Sandwich_proto.Errors.t_ProtobufError
+    -> t_ProtoBasedErrorCode
+  | ProtoBasedErrorCode_TLSConfigurationError : Sandwich_proto.Errors.t_TLSConfigurationError
+    -> t_ProtoBasedErrorCode
+  | ProtoBasedErrorCode_CertificateError : Sandwich_proto.Errors.t_CertificateError
+    -> t_ProtoBasedErrorCode
+  | ProtoBasedErrorCode_PrivateKeyError : Sandwich_proto.Errors.t_PrivateKeyError
+    -> t_ProtoBasedErrorCode
+  | ProtoBasedErrorCode_ASN1Error : Sandwich_proto.Errors.t_ASN1Error -> t_ProtoBasedErrorCode
+  | ProtoBasedErrorCode_ALPNError : Sandwich_proto.Errors.t_ALPNError -> t_ProtoBasedErrorCode
+  | ProtoBasedErrorCode_DataSourceError : Sandwich_proto.Errors.t_DataSourceError
+    -> t_ProtoBasedErrorCode
+  | ProtoBasedErrorCode_KEMError : Sandwich_proto.Errors.t_KEMError -> t_ProtoBasedErrorCode
+  | ProtoBasedErrorCode_SystemError : Sandwich_proto.Errors.t_SystemError -> t_ProtoBasedErrorCode
+  | ProtoBasedErrorCode_SocketError : Sandwich_proto.Errors.t_SocketError -> t_ProtoBasedErrorCode
+  | ProtoBasedErrorCode_HandshakeError : Sandwich_proto.Errors.t_HandshakeError
+    -> t_ProtoBasedErrorCode
+  | ProtoBasedErrorCode_TunnelError : Sandwich_proto.Errors.t_TunnelError -> t_ProtoBasedErrorCode
+
+/// Implements `[From<sandwich_proto::ErrorEnum>]` for [`ProtoBasedErrorCode`].
+[@@ FStar.Tactics.Typeclasses.tcinstance]
+val impl_9:Core.Convert.t_From t_ProtoBasedErrorCode Sandwich_proto.Errors.t_APIError
+
+/// Implements comparison operator between [`ProtoBasedErrorCode`] and the current error enum.
+[@@ FStar.Tactics.Typeclasses.tcinstance]
+val impl_16:Core.Cmp.t_PartialEq Sandwich_proto.Errors.t_APIError t_ProtoBasedErrorCode
+
+/// Implements comparison operator between [`ProtoBasedErrorCode`] and the current error enum.
+[@@ FStar.Tactics.Typeclasses.tcinstance]
+val impl_17:Core.Cmp.t_PartialEq t_ProtoBasedErrorCode Sandwich_proto.Errors.t_APIError
+
+/// Implements `[From<sandwich_proto::ErrorEnum>]` for [`ProtoBasedErrorCode`].
+[@@ FStar.Tactics.Typeclasses.tcinstance]
+val impl_18:Core.Convert.t_From t_ProtoBasedErrorCode Sandwich_proto.Errors.t_ConfigurationError
+
+/// Implements comparison operator between [`ProtoBasedErrorCode`] and the current error enum.
+[@@ FStar.Tactics.Typeclasses.tcinstance]
+val impl_25:Core.Cmp.t_PartialEq Sandwich_proto.Errors.t_ConfigurationError t_ProtoBasedErrorCode
+
+/// Implements comparison operator between [`ProtoBasedErrorCode`] and the current error enum.
+[@@ FStar.Tactics.Typeclasses.tcinstance]
+val impl_26:Core.Cmp.t_PartialEq t_ProtoBasedErrorCode Sandwich_proto.Errors.t_ConfigurationError
+
+/// Implements `[From<sandwich_proto::ErrorEnum>]` for [`ProtoBasedErrorCode`].
+[@@ FStar.Tactics.Typeclasses.tcinstance]
+val impl_27:Core.Convert.t_From t_ProtoBasedErrorCode Sandwich_proto.Errors.t_ProtobufError
+
+/// Implements comparison operator between [`ProtoBasedErrorCode`] and the current error enum.
+[@@ FStar.Tactics.Typeclasses.tcinstance]
+val impl_34:Core.Cmp.t_PartialEq Sandwich_proto.Errors.t_ProtobufError t_ProtoBasedErrorCode
+
+/// Implements comparison operator between [`ProtoBasedErrorCode`] and the current error enum.
+[@@ FStar.Tactics.Typeclasses.tcinstance]
+val impl_35:Core.Cmp.t_PartialEq t_ProtoBasedErrorCode Sandwich_proto.Errors.t_ProtobufError
+
+/// Implements `[From<sandwich_proto::ErrorEnum>]` for [`ProtoBasedErrorCode`].
+[@@ FStar.Tactics.Typeclasses.tcinstance]
+val impl_36:Core.Convert.t_From t_ProtoBasedErrorCode Sandwich_proto.Errors.t_TLSConfigurationError
+
+/// Implements comparison operator between [`ProtoBasedErrorCode`] and the current error enum.
+[@@ FStar.Tactics.Typeclasses.tcinstance]
+val impl_43:Core.Cmp.t_PartialEq Sandwich_proto.Errors.t_TLSConfigurationError t_ProtoBasedErrorCode
+
+/// Implements comparison operator between [`ProtoBasedErrorCode`] and the current error enum.
+[@@ FStar.Tactics.Typeclasses.tcinstance]
+val impl_44:Core.Cmp.t_PartialEq t_ProtoBasedErrorCode Sandwich_proto.Errors.t_TLSConfigurationError
+
+/// Implements `[From<sandwich_proto::ErrorEnum>]` for [`ProtoBasedErrorCode`].
+[@@ FStar.Tactics.Typeclasses.tcinstance]
+val impl_45:Core.Convert.t_From t_ProtoBasedErrorCode Sandwich_proto.Errors.t_CertificateError
+
+/// Implements comparison operator between [`ProtoBasedErrorCode`] and the current error enum.
+[@@ FStar.Tactics.Typeclasses.tcinstance]
+val impl_52:Core.Cmp.t_PartialEq Sandwich_proto.Errors.t_CertificateError t_ProtoBasedErrorCode
+
+/// Implements comparison operator between [`ProtoBasedErrorCode`] and the current error enum.
+[@@ FStar.Tactics.Typeclasses.tcinstance]
+val impl_53:Core.Cmp.t_PartialEq t_ProtoBasedErrorCode Sandwich_proto.Errors.t_CertificateError
+
+/// Implements `[From<sandwich_proto::ErrorEnum>]` for [`ProtoBasedErrorCode`].
+[@@ FStar.Tactics.Typeclasses.tcinstance]
+val impl_54:Core.Convert.t_From t_ProtoBasedErrorCode Sandwich_proto.Errors.t_PrivateKeyError
+
+/// Implements comparison operator between [`ProtoBasedErrorCode`] and the current error enum.
+[@@ FStar.Tactics.Typeclasses.tcinstance]
+val impl_61:Core.Cmp.t_PartialEq Sandwich_proto.Errors.t_PrivateKeyError t_ProtoBasedErrorCode
+
+/// Implements comparison operator between [`ProtoBasedErrorCode`] and the current error enum.
+[@@ FStar.Tactics.Typeclasses.tcinstance]
+val impl_62:Core.Cmp.t_PartialEq t_ProtoBasedErrorCode Sandwich_proto.Errors.t_PrivateKeyError
+
+/// Implements `[From<sandwich_proto::ErrorEnum>]` for [`ProtoBasedErrorCode`].
+[@@ FStar.Tactics.Typeclasses.tcinstance]
+val impl_63:Core.Convert.t_From t_ProtoBasedErrorCode Sandwich_proto.Errors.t_ASN1Error
+
+/// Implements comparison operator between [`ProtoBasedErrorCode`] and the current error enum.
+[@@ FStar.Tactics.Typeclasses.tcinstance]
+val impl_70:Core.Cmp.t_PartialEq Sandwich_proto.Errors.t_ASN1Error t_ProtoBasedErrorCode
+
+/// Implements comparison operator between [`ProtoBasedErrorCode`] and the current error enum.
+[@@ FStar.Tactics.Typeclasses.tcinstance]
+val impl_71:Core.Cmp.t_PartialEq t_ProtoBasedErrorCode Sandwich_proto.Errors.t_ASN1Error
+
+/// Implements `[From<sandwich_proto::ErrorEnum>]` for [`ProtoBasedErrorCode`].
+[@@ FStar.Tactics.Typeclasses.tcinstance]
+val impl_72:Core.Convert.t_From t_ProtoBasedErrorCode Sandwich_proto.Errors.t_ALPNError
+
+/// Implements comparison operator between [`ProtoBasedErrorCode`] and the current error enum.
+[@@ FStar.Tactics.Typeclasses.tcinstance]
+val impl_79:Core.Cmp.t_PartialEq Sandwich_proto.Errors.t_ALPNError t_ProtoBasedErrorCode
+
+/// Implements comparison operator between [`ProtoBasedErrorCode`] and the current error enum.
+[@@ FStar.Tactics.Typeclasses.tcinstance]
+val impl_80:Core.Cmp.t_PartialEq t_ProtoBasedErrorCode Sandwich_proto.Errors.t_ALPNError
+
+/// Implements `[From<sandwich_proto::ErrorEnum>]` for [`ProtoBasedErrorCode`].
+[@@ FStar.Tactics.Typeclasses.tcinstance]
+val impl_81:Core.Convert.t_From t_ProtoBasedErrorCode Sandwich_proto.Errors.t_DataSourceError
+
+/// Implements comparison operator between [`ProtoBasedErrorCode`] and the current error enum.
+[@@ FStar.Tactics.Typeclasses.tcinstance]
+val impl_88:Core.Cmp.t_PartialEq Sandwich_proto.Errors.t_DataSourceError t_ProtoBasedErrorCode
+
+/// Implements comparison operator between [`ProtoBasedErrorCode`] and the current error enum.
+[@@ FStar.Tactics.Typeclasses.tcinstance]
+val impl_89:Core.Cmp.t_PartialEq t_ProtoBasedErrorCode Sandwich_proto.Errors.t_DataSourceError
+
+/// Implements `[From<sandwich_proto::ErrorEnum>]` for [`ProtoBasedErrorCode`].
+[@@ FStar.Tactics.Typeclasses.tcinstance]
+val impl_90:Core.Convert.t_From t_ProtoBasedErrorCode Sandwich_proto.Errors.t_KEMError
+
+/// Implements comparison operator between [`ProtoBasedErrorCode`] and the current error enum.
+[@@ FStar.Tactics.Typeclasses.tcinstance]
+val impl_97:Core.Cmp.t_PartialEq Sandwich_proto.Errors.t_KEMError t_ProtoBasedErrorCode
+
+/// Implements comparison operator between [`ProtoBasedErrorCode`] and the current error enum.
+[@@ FStar.Tactics.Typeclasses.tcinstance]
+val impl_98:Core.Cmp.t_PartialEq t_ProtoBasedErrorCode Sandwich_proto.Errors.t_KEMError
+
+/// Implements `[From<sandwich_proto::ErrorEnum>]` for [`ProtoBasedErrorCode`].
+[@@ FStar.Tactics.Typeclasses.tcinstance]
+val impl_99:Core.Convert.t_From t_ProtoBasedErrorCode Sandwich_proto.Errors.t_SystemError
+
+/// Implements comparison operator between [`ProtoBasedErrorCode`] and the current error enum.
+[@@ FStar.Tactics.Typeclasses.tcinstance]
+val impl_106:Core.Cmp.t_PartialEq Sandwich_proto.Errors.t_SystemError t_ProtoBasedErrorCode
+
+/// Implements comparison operator between [`ProtoBasedErrorCode`] and the current error enum.
+[@@ FStar.Tactics.Typeclasses.tcinstance]
+val impl_107:Core.Cmp.t_PartialEq t_ProtoBasedErrorCode Sandwich_proto.Errors.t_SystemError
+
+/// Implements `[From<sandwich_proto::ErrorEnum>]` for [`ProtoBasedErrorCode`].
+[@@ FStar.Tactics.Typeclasses.tcinstance]
+val impl_108:Core.Convert.t_From t_ProtoBasedErrorCode Sandwich_proto.Errors.t_SocketError
+
+/// Implements comparison operator between [`ProtoBasedErrorCode`] and the current error enum.
+[@@ FStar.Tactics.Typeclasses.tcinstance]
+val impl_115:Core.Cmp.t_PartialEq Sandwich_proto.Errors.t_SocketError t_ProtoBasedErrorCode
+
+/// Implements comparison operator between [`ProtoBasedErrorCode`] and the current error enum.
+[@@ FStar.Tactics.Typeclasses.tcinstance]
+val impl_116:Core.Cmp.t_PartialEq t_ProtoBasedErrorCode Sandwich_proto.Errors.t_SocketError
+
+/// Implements `[From<sandwich_proto::ErrorEnum>]` for [`ProtoBasedErrorCode`].
+[@@ FStar.Tactics.Typeclasses.tcinstance]
+val impl_117:Core.Convert.t_From t_ProtoBasedErrorCode Sandwich_proto.Errors.t_HandshakeError
+
+/// Implements comparison operator between [`ProtoBasedErrorCode`] and the current error enum.
+[@@ FStar.Tactics.Typeclasses.tcinstance]
+val impl_124:Core.Cmp.t_PartialEq Sandwich_proto.Errors.t_HandshakeError t_ProtoBasedErrorCode
+
+/// Implements comparison operator between [`ProtoBasedErrorCode`] and the current error enum.
+[@@ FStar.Tactics.Typeclasses.tcinstance]
+val impl_125:Core.Cmp.t_PartialEq t_ProtoBasedErrorCode Sandwich_proto.Errors.t_HandshakeError
+
+/// Implements `[From<sandwich_proto::ErrorEnum>]` for [`ProtoBasedErrorCode`].
+[@@ FStar.Tactics.Typeclasses.tcinstance]
+val impl_126:Core.Convert.t_From t_ProtoBasedErrorCode Sandwich_proto.Errors.t_TunnelError
+
+/// Implements comparison operator between [`ProtoBasedErrorCode`] and the current error enum.
+[@@ FStar.Tactics.Typeclasses.tcinstance]
+val impl_133:Core.Cmp.t_PartialEq Sandwich_proto.Errors.t_TunnelError t_ProtoBasedErrorCode
+
+/// Implements comparison operator between [`ProtoBasedErrorCode`] and the current error enum.
+[@@ FStar.Tactics.Typeclasses.tcinstance]
+val impl_134:Core.Cmp.t_PartialEq t_ProtoBasedErrorCode Sandwich_proto.Errors.t_TunnelError
+
+/// Implements `Into<sandwich_proto::ErrorKind>` for [`ProtoBasedErrorCode`].
+[@@ FStar.Tactics.Typeclasses.tcinstance]
+val impl_135:Core.Convert.t_From Sandwich_proto.Errors.t_ErrorKind t_ProtoBasedErrorCode
+
 /// Implements [`std::fmt::Display`] for [`ProtoBasedErrorCode`].
 [@@ FStar.Tactics.Typeclasses.tcinstance]
-val impl_136:Core.Fmt.t_Display #t_ProtoBasedErrorCode
+val impl_136:Core.Fmt.t_Display t_ProtoBasedErrorCode
 
 /// Implements [`Into<(i32, i32)>`] for [`ProtoBasedErrorCode`].
 /// The first `i32` is the error kind, the second one is the error code.
 [@@ FStar.Tactics.Typeclasses.tcinstance]
-val impl_139:Core.Convert.t_From #(i32 & i32) #t_ProtoBasedErrorCode
-
-/// Implements `[From<sandwich_proto::ErrorEnum>]` for [`ProtoBasedErrorCode`].
-[@@ FStar.Tactics.Typeclasses.tcinstance]
-val impl_72:Core.Convert.t_From #t_ProtoBasedErrorCode #Sandwich_proto.Errors.t_ALPNError
-
-/// Adds `ErrorEnum` to the list of [`AllowedProtoBasedErrorCodeEnum`] trait.
-[@@ FStar.Tactics.Typeclasses.tcinstance]
-val impl_77:t_AllowedProtoBasedErrorCodeEnum #Sandwich_proto.Errors.t_ALPNError
-
-[@@ FStar.Tactics.Typeclasses.tcinstance]
-val impl_78:t_AllowedProtoBasedErrorCodeEnum #Sandwich_proto.Errors.t_ALPNError
-
-/// Implements comparison operator between [`ProtoBasedErrorCode`] and the current error enum.
-[@@ FStar.Tactics.Typeclasses.tcinstance]
-val impl_79:Core.Cmp.t_PartialEq #Sandwich_proto.Errors.t_ALPNError #t_ProtoBasedErrorCode
-
-/// Implements comparison operator between [`ProtoBasedErrorCode`] and the current error enum.
-[@@ FStar.Tactics.Typeclasses.tcinstance]
-val impl_80:Core.Cmp.t_PartialEq #t_ProtoBasedErrorCode #Sandwich_proto.Errors.t_ALPNError
-
-/// Implements `[From<sandwich_proto::ErrorEnum>]` for [`ProtoBasedErrorCode`].
-[@@ FStar.Tactics.Typeclasses.tcinstance]
-val impl_9:Core.Convert.t_From #t_ProtoBasedErrorCode #Sandwich_proto.Errors.t_APIError
-
-/// Adds `ErrorEnum` to the list of [`AllowedProtoBasedErrorCodeEnum`] trait.
-[@@ FStar.Tactics.Typeclasses.tcinstance]
-val impl_14:t_AllowedProtoBasedErrorCodeEnum #Sandwich_proto.Errors.t_APIError
-
-[@@ FStar.Tactics.Typeclasses.tcinstance]
-val impl_15:t_AllowedProtoBasedErrorCodeEnum #Sandwich_proto.Errors.t_APIError
-
-/// Implements comparison operator between [`ProtoBasedErrorCode`] and the current error enum.
-[@@ FStar.Tactics.Typeclasses.tcinstance]
-val impl_16:Core.Cmp.t_PartialEq #Sandwich_proto.Errors.t_APIError #t_ProtoBasedErrorCode
-
-/// Implements comparison operator between [`ProtoBasedErrorCode`] and the current error enum.
-[@@ FStar.Tactics.Typeclasses.tcinstance]
-val impl_17:Core.Cmp.t_PartialEq #t_ProtoBasedErrorCode #Sandwich_proto.Errors.t_APIError
-
-/// Implements `[From<sandwich_proto::ErrorEnum>]` for [`ProtoBasedErrorCode`].
-[@@ FStar.Tactics.Typeclasses.tcinstance]
-val impl_63:Core.Convert.t_From #t_ProtoBasedErrorCode #Sandwich_proto.Errors.t_ASN1Error
-
-/// Adds `ErrorEnum` to the list of [`AllowedProtoBasedErrorCodeEnum`] trait.
-[@@ FStar.Tactics.Typeclasses.tcinstance]
-val impl_68:t_AllowedProtoBasedErrorCodeEnum #Sandwich_proto.Errors.t_ASN1Error
-
-[@@ FStar.Tactics.Typeclasses.tcinstance]
-val impl_69:t_AllowedProtoBasedErrorCodeEnum #Sandwich_proto.Errors.t_ASN1Error
-
-/// Implements comparison operator between [`ProtoBasedErrorCode`] and the current error enum.
-[@@ FStar.Tactics.Typeclasses.tcinstance]
-val impl_70:Core.Cmp.t_PartialEq #Sandwich_proto.Errors.t_ASN1Error #t_ProtoBasedErrorCode
-
-/// Implements comparison operator between [`ProtoBasedErrorCode`] and the current error enum.
-[@@ FStar.Tactics.Typeclasses.tcinstance]
-val impl_71:Core.Cmp.t_PartialEq #t_ProtoBasedErrorCode #Sandwich_proto.Errors.t_ASN1Error
-
-/// Implements `[From<sandwich_proto::ErrorEnum>]` for [`ProtoBasedErrorCode`].
-[@@ FStar.Tactics.Typeclasses.tcinstance]
-val impl_45:Core.Convert.t_From #t_ProtoBasedErrorCode #Sandwich_proto.Errors.t_CertificateError
-
-/// Adds `ErrorEnum` to the list of [`AllowedProtoBasedErrorCodeEnum`] trait.
-[@@ FStar.Tactics.Typeclasses.tcinstance]
-val impl_50:t_AllowedProtoBasedErrorCodeEnum #Sandwich_proto.Errors.t_CertificateError
-
-[@@ FStar.Tactics.Typeclasses.tcinstance]
-val impl_51:t_AllowedProtoBasedErrorCodeEnum #Sandwich_proto.Errors.t_CertificateError
-
-/// Implements comparison operator between [`ProtoBasedErrorCode`] and the current error enum.
-[@@ FStar.Tactics.Typeclasses.tcinstance]
-val impl_52:Core.Cmp.t_PartialEq #Sandwich_proto.Errors.t_CertificateError #t_ProtoBasedErrorCode
-
-/// Implements comparison operator between [`ProtoBasedErrorCode`] and the current error enum.
-[@@ FStar.Tactics.Typeclasses.tcinstance]
-val impl_53:Core.Cmp.t_PartialEq #t_ProtoBasedErrorCode #Sandwich_proto.Errors.t_CertificateError
-
-/// Implements `[From<sandwich_proto::ErrorEnum>]` for [`ProtoBasedErrorCode`].
-[@@ FStar.Tactics.Typeclasses.tcinstance]
-val impl_18:Core.Convert.t_From #t_ProtoBasedErrorCode #Sandwich_proto.Errors.t_ConfigurationError
-
-/// Adds `ErrorEnum` to the list of [`AllowedProtoBasedErrorCodeEnum`] trait.
-[@@ FStar.Tactics.Typeclasses.tcinstance]
-val impl_23:t_AllowedProtoBasedErrorCodeEnum #Sandwich_proto.Errors.t_ConfigurationError
-
-[@@ FStar.Tactics.Typeclasses.tcinstance]
-val impl_24:t_AllowedProtoBasedErrorCodeEnum #Sandwich_proto.Errors.t_ConfigurationError
-
-/// Implements comparison operator between [`ProtoBasedErrorCode`] and the current error enum.
-[@@ FStar.Tactics.Typeclasses.tcinstance]
-val impl_25:Core.Cmp.t_PartialEq #Sandwich_proto.Errors.t_ConfigurationError #t_ProtoBasedErrorCode
-
-/// Implements comparison operator between [`ProtoBasedErrorCode`] and the current error enum.
-[@@ FStar.Tactics.Typeclasses.tcinstance]
-val impl_26:Core.Cmp.t_PartialEq #t_ProtoBasedErrorCode #Sandwich_proto.Errors.t_ConfigurationError
-
-/// Implements `[From<sandwich_proto::ErrorEnum>]` for [`ProtoBasedErrorCode`].
-[@@ FStar.Tactics.Typeclasses.tcinstance]
-val impl_81:Core.Convert.t_From #t_ProtoBasedErrorCode #Sandwich_proto.Errors.t_DataSourceError
-
-/// Adds `ErrorEnum` to the list of [`AllowedProtoBasedErrorCodeEnum`] trait.
-[@@ FStar.Tactics.Typeclasses.tcinstance]
-val impl_86:t_AllowedProtoBasedErrorCodeEnum #Sandwich_proto.Errors.t_DataSourceError
-
-[@@ FStar.Tactics.Typeclasses.tcinstance]
-val impl_87:t_AllowedProtoBasedErrorCodeEnum #Sandwich_proto.Errors.t_DataSourceError
-
-/// Implements comparison operator between [`ProtoBasedErrorCode`] and the current error enum.
-[@@ FStar.Tactics.Typeclasses.tcinstance]
-val impl_88:Core.Cmp.t_PartialEq #Sandwich_proto.Errors.t_DataSourceError #t_ProtoBasedErrorCode
-
-/// Implements comparison operator between [`ProtoBasedErrorCode`] and the current error enum.
-[@@ FStar.Tactics.Typeclasses.tcinstance]
-val impl_89:Core.Cmp.t_PartialEq #t_ProtoBasedErrorCode #Sandwich_proto.Errors.t_DataSourceError
-
-/// Implements `Into<sandwich_proto::ErrorKind>` for [`ProtoBasedErrorCode`].
-[@@ FStar.Tactics.Typeclasses.tcinstance]
-val impl_135:Core.Convert.t_From #Sandwich_proto.Errors.t_ErrorKind #t_ProtoBasedErrorCode
-
-/// Implements `[From<sandwich_proto::ErrorEnum>]` for [`ProtoBasedErrorCode`].
-[@@ FStar.Tactics.Typeclasses.tcinstance]
-val impl_117:Core.Convert.t_From #t_ProtoBasedErrorCode #Sandwich_proto.Errors.t_HandshakeError
-
-/// Adds `ErrorEnum` to the list of [`AllowedProtoBasedErrorCodeEnum`] trait.
-[@@ FStar.Tactics.Typeclasses.tcinstance]
-val impl_122:t_AllowedProtoBasedErrorCodeEnum #Sandwich_proto.Errors.t_HandshakeError
-
-[@@ FStar.Tactics.Typeclasses.tcinstance]
-val impl_123:t_AllowedProtoBasedErrorCodeEnum #Sandwich_proto.Errors.t_HandshakeError
-
-/// Implements comparison operator between [`ProtoBasedErrorCode`] and the current error enum.
-[@@ FStar.Tactics.Typeclasses.tcinstance]
-val impl_124:Core.Cmp.t_PartialEq #Sandwich_proto.Errors.t_HandshakeError #t_ProtoBasedErrorCode
-
-/// Implements comparison operator between [`ProtoBasedErrorCode`] and the current error enum.
-[@@ FStar.Tactics.Typeclasses.tcinstance]
-val impl_125:Core.Cmp.t_PartialEq #t_ProtoBasedErrorCode #Sandwich_proto.Errors.t_HandshakeError
-
-/// Implements `[From<sandwich_proto::ErrorEnum>]` for [`ProtoBasedErrorCode`].
-[@@ FStar.Tactics.Typeclasses.tcinstance]
-val impl_90:Core.Convert.t_From #t_ProtoBasedErrorCode #Sandwich_proto.Errors.t_KEMError
-
-/// Adds `ErrorEnum` to the list of [`AllowedProtoBasedErrorCodeEnum`] trait.
-[@@ FStar.Tactics.Typeclasses.tcinstance]
-val impl_95:t_AllowedProtoBasedErrorCodeEnum #Sandwich_proto.Errors.t_KEMError
-
-[@@ FStar.Tactics.Typeclasses.tcinstance]
-val impl_96:t_AllowedProtoBasedErrorCodeEnum #Sandwich_proto.Errors.t_KEMError
-
-/// Implements comparison operator between [`ProtoBasedErrorCode`] and the current error enum.
-[@@ FStar.Tactics.Typeclasses.tcinstance]
-val impl_97:Core.Cmp.t_PartialEq #Sandwich_proto.Errors.t_KEMError #t_ProtoBasedErrorCode
-
-/// Implements comparison operator between [`ProtoBasedErrorCode`] and the current error enum.
-[@@ FStar.Tactics.Typeclasses.tcinstance]
-val impl_98:Core.Cmp.t_PartialEq #t_ProtoBasedErrorCode #Sandwich_proto.Errors.t_KEMError
-
-/// Implements `[From<sandwich_proto::ErrorEnum>]` for [`ProtoBasedErrorCode`].
-[@@ FStar.Tactics.Typeclasses.tcinstance]
-val impl_54:Core.Convert.t_From #t_ProtoBasedErrorCode #Sandwich_proto.Errors.t_PrivateKeyError
-
-/// Adds `ErrorEnum` to the list of [`AllowedProtoBasedErrorCodeEnum`] trait.
-[@@ FStar.Tactics.Typeclasses.tcinstance]
-val impl_59:t_AllowedProtoBasedErrorCodeEnum #Sandwich_proto.Errors.t_PrivateKeyError
-
-[@@ FStar.Tactics.Typeclasses.tcinstance]
-val impl_60:t_AllowedProtoBasedErrorCodeEnum #Sandwich_proto.Errors.t_PrivateKeyError
-
-/// Implements comparison operator between [`ProtoBasedErrorCode`] and the current error enum.
-[@@ FStar.Tactics.Typeclasses.tcinstance]
-val impl_61:Core.Cmp.t_PartialEq #Sandwich_proto.Errors.t_PrivateKeyError #t_ProtoBasedErrorCode
-
-/// Implements comparison operator between [`ProtoBasedErrorCode`] and the current error enum.
-[@@ FStar.Tactics.Typeclasses.tcinstance]
-val impl_62:Core.Cmp.t_PartialEq #t_ProtoBasedErrorCode #Sandwich_proto.Errors.t_PrivateKeyError
-
-/// Implements `[From<sandwich_proto::ErrorEnum>]` for [`ProtoBasedErrorCode`].
-[@@ FStar.Tactics.Typeclasses.tcinstance]
-val impl_27:Core.Convert.t_From #t_ProtoBasedErrorCode #Sandwich_proto.Errors.t_ProtobufError
-
-/// Adds `ErrorEnum` to the list of [`AllowedProtoBasedErrorCodeEnum`] trait.
-[@@ FStar.Tactics.Typeclasses.tcinstance]
-val impl_32:t_AllowedProtoBasedErrorCodeEnum #Sandwich_proto.Errors.t_ProtobufError
-
-[@@ FStar.Tactics.Typeclasses.tcinstance]
-val impl_33:t_AllowedProtoBasedErrorCodeEnum #Sandwich_proto.Errors.t_ProtobufError
-
-/// Implements comparison operator between [`ProtoBasedErrorCode`] and the current error enum.
-[@@ FStar.Tactics.Typeclasses.tcinstance]
-val impl_34:Core.Cmp.t_PartialEq #Sandwich_proto.Errors.t_ProtobufError #t_ProtoBasedErrorCode
-
-/// Implements comparison operator between [`ProtoBasedErrorCode`] and the current error enum.
-[@@ FStar.Tactics.Typeclasses.tcinstance]
-val impl_35:Core.Cmp.t_PartialEq #t_ProtoBasedErrorCode #Sandwich_proto.Errors.t_ProtobufError
-
-/// Implements `[From<sandwich_proto::ErrorEnum>]` for [`ProtoBasedErrorCode`].
-[@@ FStar.Tactics.Typeclasses.tcinstance]
-val impl_108:Core.Convert.t_From #t_ProtoBasedErrorCode #Sandwich_proto.Errors.t_SocketError
-
-/// Adds `ErrorEnum` to the list of [`AllowedProtoBasedErrorCodeEnum`] trait.
-[@@ FStar.Tactics.Typeclasses.tcinstance]
-val impl_113:t_AllowedProtoBasedErrorCodeEnum #Sandwich_proto.Errors.t_SocketError
-
-[@@ FStar.Tactics.Typeclasses.tcinstance]
-val impl_114:t_AllowedProtoBasedErrorCodeEnum #Sandwich_proto.Errors.t_SocketError
-
-/// Implements comparison operator between [`ProtoBasedErrorCode`] and the current error enum.
-[@@ FStar.Tactics.Typeclasses.tcinstance]
-val impl_115:Core.Cmp.t_PartialEq #Sandwich_proto.Errors.t_SocketError #t_ProtoBasedErrorCode
-
-/// Implements comparison operator between [`ProtoBasedErrorCode`] and the current error enum.
-[@@ FStar.Tactics.Typeclasses.tcinstance]
-val impl_116:Core.Cmp.t_PartialEq #t_ProtoBasedErrorCode #Sandwich_proto.Errors.t_SocketError
-
-/// Implements `[From<sandwich_proto::ErrorEnum>]` for [`ProtoBasedErrorCode`].
-[@@ FStar.Tactics.Typeclasses.tcinstance]
-val impl_99:Core.Convert.t_From #t_ProtoBasedErrorCode #Sandwich_proto.Errors.t_SystemError
-
-/// Adds `ErrorEnum` to the list of [`AllowedProtoBasedErrorCodeEnum`] trait.
-[@@ FStar.Tactics.Typeclasses.tcinstance]
-val impl_104:t_AllowedProtoBasedErrorCodeEnum #Sandwich_proto.Errors.t_SystemError
-
-[@@ FStar.Tactics.Typeclasses.tcinstance]
-val impl_105:t_AllowedProtoBasedErrorCodeEnum #Sandwich_proto.Errors.t_SystemError
-
-/// Implements comparison operator between [`ProtoBasedErrorCode`] and the current error enum.
-[@@ FStar.Tactics.Typeclasses.tcinstance]
-val impl_106:Core.Cmp.t_PartialEq #Sandwich_proto.Errors.t_SystemError #t_ProtoBasedErrorCode
-
-/// Implements comparison operator between [`ProtoBasedErrorCode`] and the current error enum.
-[@@ FStar.Tactics.Typeclasses.tcinstance]
-val impl_107:Core.Cmp.t_PartialEq #t_ProtoBasedErrorCode #Sandwich_proto.Errors.t_SystemError
-
-/// Implements `[From<sandwich_proto::ErrorEnum>]` for [`ProtoBasedErrorCode`].
-[@@ FStar.Tactics.Typeclasses.tcinstance]
-val impl_36:Core.Convert.t_From #t_ProtoBasedErrorCode
-  #Sandwich_proto.Errors.t_TLSConfigurationError
-
-/// Adds `ErrorEnum` to the list of [`AllowedProtoBasedErrorCodeEnum`] trait.
-[@@ FStar.Tactics.Typeclasses.tcinstance]
-val impl_41:t_AllowedProtoBasedErrorCodeEnum #Sandwich_proto.Errors.t_TLSConfigurationError
-
-[@@ FStar.Tactics.Typeclasses.tcinstance]
-val impl_42:t_AllowedProtoBasedErrorCodeEnum #Sandwich_proto.Errors.t_TLSConfigurationError
-
-/// Implements comparison operator between [`ProtoBasedErrorCode`] and the current error enum.
-[@@ FStar.Tactics.Typeclasses.tcinstance]
-val impl_43:Core.Cmp.t_PartialEq #Sandwich_proto.Errors.t_TLSConfigurationError
-  #t_ProtoBasedErrorCode
-
-/// Implements comparison operator between [`ProtoBasedErrorCode`] and the current error enum.
-[@@ FStar.Tactics.Typeclasses.tcinstance]
-val impl_44:Core.Cmp.t_PartialEq #t_ProtoBasedErrorCode
-  #Sandwich_proto.Errors.t_TLSConfigurationError
-
-/// Implements `[From<sandwich_proto::ErrorEnum>]` for [`ProtoBasedErrorCode`].
-[@@ FStar.Tactics.Typeclasses.tcinstance]
-val impl_126:Core.Convert.t_From #t_ProtoBasedErrorCode #Sandwich_proto.Errors.t_TunnelError
-
-/// Adds `ErrorEnum` to the list of [`AllowedProtoBasedErrorCodeEnum`] trait.
-[@@ FStar.Tactics.Typeclasses.tcinstance]
-val impl_131:t_AllowedProtoBasedErrorCodeEnum #Sandwich_proto.Errors.t_TunnelError
-
-[@@ FStar.Tactics.Typeclasses.tcinstance]
-val impl_132:t_AllowedProtoBasedErrorCodeEnum #Sandwich_proto.Errors.t_TunnelError
-
-/// Implements comparison operator between [`ProtoBasedErrorCode`] and the current error enum.
-[@@ FStar.Tactics.Typeclasses.tcinstance]
-val impl_133:Core.Cmp.t_PartialEq #Sandwich_proto.Errors.t_TunnelError #t_ProtoBasedErrorCode
-
-/// Implements comparison operator between [`ProtoBasedErrorCode`] and the current error enum.
-[@@ FStar.Tactics.Typeclasses.tcinstance]
-val impl_134:Core.Cmp.t_PartialEq #t_ProtoBasedErrorCode #Sandwich_proto.Errors.t_TunnelError
+val impl_139:Core.Convert.t_From (i32 & i32) t_ProtoBasedErrorCode
 
 /// An error code.
 /// An error code consists of an error code based on a protobuf enum - [`ProtoBasedErrorCode`]
@@ -301,290 +330,289 @@ type t_ErrorCode = {
 
 /// Implements [`std::borrow::Borrow`] for [`ErrorCode`] and [`ProtoBasedErrorCode`].
 [@@ FStar.Tactics.Typeclasses.tcinstance]
-val impl:Core.Borrow.t_Borrow #t_ErrorCode #t_ProtoBasedErrorCode
+val impl:Core.Borrow.t_Borrow t_ErrorCode t_ProtoBasedErrorCode
 
 /// Implements [`std::fmt::Display`] for [`ErrorCode`].
 [@@ FStar.Tactics.Typeclasses.tcinstance]
-val impl_1:Core.Fmt.t_Display #t_ErrorCode
+val impl_1:Core.Fmt.t_Display t_ErrorCode
 
 /// Instantiates an [`ErrorCode`] by consuming a [`ProtoBasedErrorCode`].
 [@@ FStar.Tactics.Typeclasses.tcinstance]
-val impl_2:Core.Convert.t_From #t_ErrorCode #t_ProtoBasedErrorCode
+val impl_2:Core.Convert.t_From t_ErrorCode t_ProtoBasedErrorCode
 
 /// Implements [`Into<(i32, i32)>`] for [`ErrorCode`].
 /// The first `i32` is the error kind, the second one is the error code.
 [@@ FStar.Tactics.Typeclasses.tcinstance]
-val impl_4:Core.Convert.t_From #(i32 & i32) #t_ErrorCode
+val impl_4:Core.Convert.t_From (i32 & i32) t_ErrorCode
 
 [@@ FStar.Tactics.Typeclasses.tcinstance]
 val impl_5 (#v_S: Type0) {| i1: Core.Convert.t_AsRef v_S string |}
-    : Core.Convert.t_From #t_ErrorCode #(t_ProtoBasedErrorCode & v_S)
+    : Core.Convert.t_From t_ErrorCode (t_ProtoBasedErrorCode & v_S)
 
 /// Instantiates an [`ErrorCode`] by consuming a [`ProtoBasedErrorCode`] and a string.
 [@@ FStar.Tactics.Typeclasses.tcinstance]
-val impl_6:Core.Convert.t_From #t_ErrorCode #(t_ProtoBasedErrorCode & string)
+val impl_6:Core.Convert.t_From t_ErrorCode (t_ProtoBasedErrorCode & string)
 
 /// Instantiates an [`ErrorCode`] by consuming a [`ProtoBasedErrorCode`] and a string.
 [@@ FStar.Tactics.Typeclasses.tcinstance]
-val impl_7:Core.Convert.t_From #t_ErrorCode #(t_ProtoBasedErrorCode & Alloc.String.t_String)
+val impl_7:Core.Convert.t_From t_ErrorCode (t_ProtoBasedErrorCode & Alloc.String.t_String)
 
 /// Implements `[From<sandwich_proto::ErrorEnum>]` for [`ErrorCode`].
 [@@ FStar.Tactics.Typeclasses.tcinstance]
-val impl_10:Core.Convert.t_From #t_ErrorCode #Sandwich_proto.Errors.t_APIError
+val impl_10:Core.Convert.t_From t_ErrorCode Sandwich_proto.Errors.t_APIError
 
 /// Instantiates an [`ErrorCode`] from an error enum and a string.
 [@@ FStar.Tactics.Typeclasses.tcinstance]
 val impl_11 (#v_S: Type0) {| i1: Core.Convert.t_AsRef v_S string |}
-    : Core.Convert.t_From #t_ErrorCode #(Sandwich_proto.Errors.t_APIError & v_S)
+    : Core.Convert.t_From t_ErrorCode (Sandwich_proto.Errors.t_APIError & v_S)
 
 /// Instantiates an [`ErrorCode`] from an error enum and a string.
 [@@ FStar.Tactics.Typeclasses.tcinstance]
-val impl_12:Core.Convert.t_From #t_ErrorCode #(Sandwich_proto.Errors.t_APIError & string)
+val impl_12:Core.Convert.t_From t_ErrorCode (Sandwich_proto.Errors.t_APIError & string)
 
 /// Instantiates an [`ErrorCode`] from an error enum and a [`String`].
 [@@ FStar.Tactics.Typeclasses.tcinstance]
-val impl_13:Core.Convert.t_From #t_ErrorCode
-  #(Sandwich_proto.Errors.t_APIError & Alloc.String.t_String)
+val impl_13:Core.Convert.t_From t_ErrorCode
+  (Sandwich_proto.Errors.t_APIError & Alloc.String.t_String)
 
 /// Implements `[From<sandwich_proto::ErrorEnum>]` for [`ErrorCode`].
 [@@ FStar.Tactics.Typeclasses.tcinstance]
-val impl_19:Core.Convert.t_From #t_ErrorCode #Sandwich_proto.Errors.t_ConfigurationError
+val impl_19:Core.Convert.t_From t_ErrorCode Sandwich_proto.Errors.t_ConfigurationError
 
 /// Instantiates an [`ErrorCode`] from an error enum and a string.
 [@@ FStar.Tactics.Typeclasses.tcinstance]
 val impl_20 (#v_S: Type0) {| i1: Core.Convert.t_AsRef v_S string |}
-    : Core.Convert.t_From #t_ErrorCode #(Sandwich_proto.Errors.t_ConfigurationError & v_S)
+    : Core.Convert.t_From t_ErrorCode (Sandwich_proto.Errors.t_ConfigurationError & v_S)
 
 /// Instantiates an [`ErrorCode`] from an error enum and a string.
 [@@ FStar.Tactics.Typeclasses.tcinstance]
-val impl_21:Core.Convert.t_From #t_ErrorCode #(Sandwich_proto.Errors.t_ConfigurationError & string)
+val impl_21:Core.Convert.t_From t_ErrorCode (Sandwich_proto.Errors.t_ConfigurationError & string)
 
 /// Instantiates an [`ErrorCode`] from an error enum and a [`String`].
 [@@ FStar.Tactics.Typeclasses.tcinstance]
-val impl_22:Core.Convert.t_From #t_ErrorCode
-  #(Sandwich_proto.Errors.t_ConfigurationError & Alloc.String.t_String)
+val impl_22:Core.Convert.t_From t_ErrorCode
+  (Sandwich_proto.Errors.t_ConfigurationError & Alloc.String.t_String)
 
 /// Implements `[From<sandwich_proto::ErrorEnum>]` for [`ErrorCode`].
 [@@ FStar.Tactics.Typeclasses.tcinstance]
-val impl_28:Core.Convert.t_From #t_ErrorCode #Sandwich_proto.Errors.t_ProtobufError
+val impl_28:Core.Convert.t_From t_ErrorCode Sandwich_proto.Errors.t_ProtobufError
 
 /// Instantiates an [`ErrorCode`] from an error enum and a string.
 [@@ FStar.Tactics.Typeclasses.tcinstance]
 val impl_29 (#v_S: Type0) {| i1: Core.Convert.t_AsRef v_S string |}
-    : Core.Convert.t_From #t_ErrorCode #(Sandwich_proto.Errors.t_ProtobufError & v_S)
+    : Core.Convert.t_From t_ErrorCode (Sandwich_proto.Errors.t_ProtobufError & v_S)
 
 /// Instantiates an [`ErrorCode`] from an error enum and a string.
 [@@ FStar.Tactics.Typeclasses.tcinstance]
-val impl_30:Core.Convert.t_From #t_ErrorCode #(Sandwich_proto.Errors.t_ProtobufError & string)
+val impl_30:Core.Convert.t_From t_ErrorCode (Sandwich_proto.Errors.t_ProtobufError & string)
 
 /// Instantiates an [`ErrorCode`] from an error enum and a [`String`].
 [@@ FStar.Tactics.Typeclasses.tcinstance]
-val impl_31:Core.Convert.t_From #t_ErrorCode
-  #(Sandwich_proto.Errors.t_ProtobufError & Alloc.String.t_String)
+val impl_31:Core.Convert.t_From t_ErrorCode
+  (Sandwich_proto.Errors.t_ProtobufError & Alloc.String.t_String)
 
 /// Implements `[From<sandwich_proto::ErrorEnum>]` for [`ErrorCode`].
 [@@ FStar.Tactics.Typeclasses.tcinstance]
-val impl_37:Core.Convert.t_From #t_ErrorCode #Sandwich_proto.Errors.t_TLSConfigurationError
+val impl_37:Core.Convert.t_From t_ErrorCode Sandwich_proto.Errors.t_TLSConfigurationError
 
 /// Instantiates an [`ErrorCode`] from an error enum and a string.
 [@@ FStar.Tactics.Typeclasses.tcinstance]
 val impl_38 (#v_S: Type0) {| i1: Core.Convert.t_AsRef v_S string |}
-    : Core.Convert.t_From #t_ErrorCode #(Sandwich_proto.Errors.t_TLSConfigurationError & v_S)
+    : Core.Convert.t_From t_ErrorCode (Sandwich_proto.Errors.t_TLSConfigurationError & v_S)
 
 /// Instantiates an [`ErrorCode`] from an error enum and a string.
 [@@ FStar.Tactics.Typeclasses.tcinstance]
-val impl_39:Core.Convert.t_From #t_ErrorCode
-  #(Sandwich_proto.Errors.t_TLSConfigurationError & string)
+val impl_39:Core.Convert.t_From t_ErrorCode (Sandwich_proto.Errors.t_TLSConfigurationError & string)
 
 /// Instantiates an [`ErrorCode`] from an error enum and a [`String`].
 [@@ FStar.Tactics.Typeclasses.tcinstance]
-val impl_40:Core.Convert.t_From #t_ErrorCode
-  #(Sandwich_proto.Errors.t_TLSConfigurationError & Alloc.String.t_String)
+val impl_40:Core.Convert.t_From t_ErrorCode
+  (Sandwich_proto.Errors.t_TLSConfigurationError & Alloc.String.t_String)
 
 /// Implements `[From<sandwich_proto::ErrorEnum>]` for [`ErrorCode`].
 [@@ FStar.Tactics.Typeclasses.tcinstance]
-val impl_46:Core.Convert.t_From #t_ErrorCode #Sandwich_proto.Errors.t_CertificateError
+val impl_46:Core.Convert.t_From t_ErrorCode Sandwich_proto.Errors.t_CertificateError
 
 /// Instantiates an [`ErrorCode`] from an error enum and a string.
 [@@ FStar.Tactics.Typeclasses.tcinstance]
 val impl_47 (#v_S: Type0) {| i1: Core.Convert.t_AsRef v_S string |}
-    : Core.Convert.t_From #t_ErrorCode #(Sandwich_proto.Errors.t_CertificateError & v_S)
+    : Core.Convert.t_From t_ErrorCode (Sandwich_proto.Errors.t_CertificateError & v_S)
 
 /// Instantiates an [`ErrorCode`] from an error enum and a string.
 [@@ FStar.Tactics.Typeclasses.tcinstance]
-val impl_48:Core.Convert.t_From #t_ErrorCode #(Sandwich_proto.Errors.t_CertificateError & string)
+val impl_48:Core.Convert.t_From t_ErrorCode (Sandwich_proto.Errors.t_CertificateError & string)
 
 /// Instantiates an [`ErrorCode`] from an error enum and a [`String`].
 [@@ FStar.Tactics.Typeclasses.tcinstance]
-val impl_49:Core.Convert.t_From #t_ErrorCode
-  #(Sandwich_proto.Errors.t_CertificateError & Alloc.String.t_String)
+val impl_49:Core.Convert.t_From t_ErrorCode
+  (Sandwich_proto.Errors.t_CertificateError & Alloc.String.t_String)
 
 /// Implements `[From<sandwich_proto::ErrorEnum>]` for [`ErrorCode`].
 [@@ FStar.Tactics.Typeclasses.tcinstance]
-val impl_55:Core.Convert.t_From #t_ErrorCode #Sandwich_proto.Errors.t_PrivateKeyError
+val impl_55:Core.Convert.t_From t_ErrorCode Sandwich_proto.Errors.t_PrivateKeyError
 
 /// Instantiates an [`ErrorCode`] from an error enum and a string.
 [@@ FStar.Tactics.Typeclasses.tcinstance]
 val impl_56 (#v_S: Type0) {| i1: Core.Convert.t_AsRef v_S string |}
-    : Core.Convert.t_From #t_ErrorCode #(Sandwich_proto.Errors.t_PrivateKeyError & v_S)
+    : Core.Convert.t_From t_ErrorCode (Sandwich_proto.Errors.t_PrivateKeyError & v_S)
 
 /// Instantiates an [`ErrorCode`] from an error enum and a string.
 [@@ FStar.Tactics.Typeclasses.tcinstance]
-val impl_57:Core.Convert.t_From #t_ErrorCode #(Sandwich_proto.Errors.t_PrivateKeyError & string)
+val impl_57:Core.Convert.t_From t_ErrorCode (Sandwich_proto.Errors.t_PrivateKeyError & string)
 
 /// Instantiates an [`ErrorCode`] from an error enum and a [`String`].
 [@@ FStar.Tactics.Typeclasses.tcinstance]
-val impl_58:Core.Convert.t_From #t_ErrorCode
-  #(Sandwich_proto.Errors.t_PrivateKeyError & Alloc.String.t_String)
+val impl_58:Core.Convert.t_From t_ErrorCode
+  (Sandwich_proto.Errors.t_PrivateKeyError & Alloc.String.t_String)
 
 /// Implements `[From<sandwich_proto::ErrorEnum>]` for [`ErrorCode`].
 [@@ FStar.Tactics.Typeclasses.tcinstance]
-val impl_64:Core.Convert.t_From #t_ErrorCode #Sandwich_proto.Errors.t_ASN1Error
+val impl_64:Core.Convert.t_From t_ErrorCode Sandwich_proto.Errors.t_ASN1Error
 
 /// Instantiates an [`ErrorCode`] from an error enum and a string.
 [@@ FStar.Tactics.Typeclasses.tcinstance]
 val impl_65 (#v_S: Type0) {| i1: Core.Convert.t_AsRef v_S string |}
-    : Core.Convert.t_From #t_ErrorCode #(Sandwich_proto.Errors.t_ASN1Error & v_S)
+    : Core.Convert.t_From t_ErrorCode (Sandwich_proto.Errors.t_ASN1Error & v_S)
 
 /// Instantiates an [`ErrorCode`] from an error enum and a string.
 [@@ FStar.Tactics.Typeclasses.tcinstance]
-val impl_66:Core.Convert.t_From #t_ErrorCode #(Sandwich_proto.Errors.t_ASN1Error & string)
+val impl_66:Core.Convert.t_From t_ErrorCode (Sandwich_proto.Errors.t_ASN1Error & string)
 
 /// Instantiates an [`ErrorCode`] from an error enum and a [`String`].
 [@@ FStar.Tactics.Typeclasses.tcinstance]
-val impl_67:Core.Convert.t_From #t_ErrorCode
-  #(Sandwich_proto.Errors.t_ASN1Error & Alloc.String.t_String)
+val impl_67:Core.Convert.t_From t_ErrorCode
+  (Sandwich_proto.Errors.t_ASN1Error & Alloc.String.t_String)
 
 /// Implements `[From<sandwich_proto::ErrorEnum>]` for [`ErrorCode`].
 [@@ FStar.Tactics.Typeclasses.tcinstance]
-val impl_73:Core.Convert.t_From #t_ErrorCode #Sandwich_proto.Errors.t_ALPNError
+val impl_73:Core.Convert.t_From t_ErrorCode Sandwich_proto.Errors.t_ALPNError
 
 /// Instantiates an [`ErrorCode`] from an error enum and a string.
 [@@ FStar.Tactics.Typeclasses.tcinstance]
 val impl_74 (#v_S: Type0) {| i1: Core.Convert.t_AsRef v_S string |}
-    : Core.Convert.t_From #t_ErrorCode #(Sandwich_proto.Errors.t_ALPNError & v_S)
+    : Core.Convert.t_From t_ErrorCode (Sandwich_proto.Errors.t_ALPNError & v_S)
 
 /// Instantiates an [`ErrorCode`] from an error enum and a string.
 [@@ FStar.Tactics.Typeclasses.tcinstance]
-val impl_75:Core.Convert.t_From #t_ErrorCode #(Sandwich_proto.Errors.t_ALPNError & string)
+val impl_75:Core.Convert.t_From t_ErrorCode (Sandwich_proto.Errors.t_ALPNError & string)
 
 /// Instantiates an [`ErrorCode`] from an error enum and a [`String`].
 [@@ FStar.Tactics.Typeclasses.tcinstance]
-val impl_76:Core.Convert.t_From #t_ErrorCode
-  #(Sandwich_proto.Errors.t_ALPNError & Alloc.String.t_String)
+val impl_76:Core.Convert.t_From t_ErrorCode
+  (Sandwich_proto.Errors.t_ALPNError & Alloc.String.t_String)
 
 /// Implements `[From<sandwich_proto::ErrorEnum>]` for [`ErrorCode`].
 [@@ FStar.Tactics.Typeclasses.tcinstance]
-val impl_82:Core.Convert.t_From #t_ErrorCode #Sandwich_proto.Errors.t_DataSourceError
+val impl_82:Core.Convert.t_From t_ErrorCode Sandwich_proto.Errors.t_DataSourceError
 
 /// Instantiates an [`ErrorCode`] from an error enum and a string.
 [@@ FStar.Tactics.Typeclasses.tcinstance]
 val impl_83 (#v_S: Type0) {| i1: Core.Convert.t_AsRef v_S string |}
-    : Core.Convert.t_From #t_ErrorCode #(Sandwich_proto.Errors.t_DataSourceError & v_S)
+    : Core.Convert.t_From t_ErrorCode (Sandwich_proto.Errors.t_DataSourceError & v_S)
 
 /// Instantiates an [`ErrorCode`] from an error enum and a string.
 [@@ FStar.Tactics.Typeclasses.tcinstance]
-val impl_84:Core.Convert.t_From #t_ErrorCode #(Sandwich_proto.Errors.t_DataSourceError & string)
+val impl_84:Core.Convert.t_From t_ErrorCode (Sandwich_proto.Errors.t_DataSourceError & string)
 
 /// Instantiates an [`ErrorCode`] from an error enum and a [`String`].
 [@@ FStar.Tactics.Typeclasses.tcinstance]
-val impl_85:Core.Convert.t_From #t_ErrorCode
-  #(Sandwich_proto.Errors.t_DataSourceError & Alloc.String.t_String)
+val impl_85:Core.Convert.t_From t_ErrorCode
+  (Sandwich_proto.Errors.t_DataSourceError & Alloc.String.t_String)
 
 /// Implements `[From<sandwich_proto::ErrorEnum>]` for [`ErrorCode`].
 [@@ FStar.Tactics.Typeclasses.tcinstance]
-val impl_91:Core.Convert.t_From #t_ErrorCode #Sandwich_proto.Errors.t_KEMError
+val impl_91:Core.Convert.t_From t_ErrorCode Sandwich_proto.Errors.t_KEMError
 
 /// Instantiates an [`ErrorCode`] from an error enum and a string.
 [@@ FStar.Tactics.Typeclasses.tcinstance]
 val impl_92 (#v_S: Type0) {| i1: Core.Convert.t_AsRef v_S string |}
-    : Core.Convert.t_From #t_ErrorCode #(Sandwich_proto.Errors.t_KEMError & v_S)
+    : Core.Convert.t_From t_ErrorCode (Sandwich_proto.Errors.t_KEMError & v_S)
 
 /// Instantiates an [`ErrorCode`] from an error enum and a string.
 [@@ FStar.Tactics.Typeclasses.tcinstance]
-val impl_93:Core.Convert.t_From #t_ErrorCode #(Sandwich_proto.Errors.t_KEMError & string)
+val impl_93:Core.Convert.t_From t_ErrorCode (Sandwich_proto.Errors.t_KEMError & string)
 
 /// Instantiates an [`ErrorCode`] from an error enum and a [`String`].
 [@@ FStar.Tactics.Typeclasses.tcinstance]
-val impl_94:Core.Convert.t_From #t_ErrorCode
-  #(Sandwich_proto.Errors.t_KEMError & Alloc.String.t_String)
+val impl_94:Core.Convert.t_From t_ErrorCode
+  (Sandwich_proto.Errors.t_KEMError & Alloc.String.t_String)
 
 /// Implements `[From<sandwich_proto::ErrorEnum>]` for [`ErrorCode`].
 [@@ FStar.Tactics.Typeclasses.tcinstance]
-val impl_100:Core.Convert.t_From #t_ErrorCode #Sandwich_proto.Errors.t_SystemError
+val impl_100:Core.Convert.t_From t_ErrorCode Sandwich_proto.Errors.t_SystemError
 
 /// Instantiates an [`ErrorCode`] from an error enum and a string.
 [@@ FStar.Tactics.Typeclasses.tcinstance]
 val impl_101 (#v_S: Type0) {| i1: Core.Convert.t_AsRef v_S string |}
-    : Core.Convert.t_From #t_ErrorCode #(Sandwich_proto.Errors.t_SystemError & v_S)
+    : Core.Convert.t_From t_ErrorCode (Sandwich_proto.Errors.t_SystemError & v_S)
 
 /// Instantiates an [`ErrorCode`] from an error enum and a string.
 [@@ FStar.Tactics.Typeclasses.tcinstance]
-val impl_102:Core.Convert.t_From #t_ErrorCode #(Sandwich_proto.Errors.t_SystemError & string)
+val impl_102:Core.Convert.t_From t_ErrorCode (Sandwich_proto.Errors.t_SystemError & string)
 
 /// Instantiates an [`ErrorCode`] from an error enum and a [`String`].
 [@@ FStar.Tactics.Typeclasses.tcinstance]
-val impl_103:Core.Convert.t_From #t_ErrorCode
-  #(Sandwich_proto.Errors.t_SystemError & Alloc.String.t_String)
+val impl_103:Core.Convert.t_From t_ErrorCode
+  (Sandwich_proto.Errors.t_SystemError & Alloc.String.t_String)
 
 /// Implements `[From<sandwich_proto::ErrorEnum>]` for [`ErrorCode`].
 [@@ FStar.Tactics.Typeclasses.tcinstance]
-val impl_109:Core.Convert.t_From #t_ErrorCode #Sandwich_proto.Errors.t_SocketError
+val impl_109:Core.Convert.t_From t_ErrorCode Sandwich_proto.Errors.t_SocketError
 
 /// Instantiates an [`ErrorCode`] from an error enum and a string.
 [@@ FStar.Tactics.Typeclasses.tcinstance]
 val impl_110 (#v_S: Type0) {| i1: Core.Convert.t_AsRef v_S string |}
-    : Core.Convert.t_From #t_ErrorCode #(Sandwich_proto.Errors.t_SocketError & v_S)
+    : Core.Convert.t_From t_ErrorCode (Sandwich_proto.Errors.t_SocketError & v_S)
 
 /// Instantiates an [`ErrorCode`] from an error enum and a string.
 [@@ FStar.Tactics.Typeclasses.tcinstance]
-val impl_111:Core.Convert.t_From #t_ErrorCode #(Sandwich_proto.Errors.t_SocketError & string)
+val impl_111:Core.Convert.t_From t_ErrorCode (Sandwich_proto.Errors.t_SocketError & string)
 
 /// Instantiates an [`ErrorCode`] from an error enum and a [`String`].
 [@@ FStar.Tactics.Typeclasses.tcinstance]
-val impl_112:Core.Convert.t_From #t_ErrorCode
-  #(Sandwich_proto.Errors.t_SocketError & Alloc.String.t_String)
+val impl_112:Core.Convert.t_From t_ErrorCode
+  (Sandwich_proto.Errors.t_SocketError & Alloc.String.t_String)
 
 /// Implements `[From<sandwich_proto::ErrorEnum>]` for [`ErrorCode`].
 [@@ FStar.Tactics.Typeclasses.tcinstance]
-val impl_118:Core.Convert.t_From #t_ErrorCode #Sandwich_proto.Errors.t_HandshakeError
+val impl_118:Core.Convert.t_From t_ErrorCode Sandwich_proto.Errors.t_HandshakeError
 
 /// Instantiates an [`ErrorCode`] from an error enum and a string.
 [@@ FStar.Tactics.Typeclasses.tcinstance]
 val impl_119 (#v_S: Type0) {| i1: Core.Convert.t_AsRef v_S string |}
-    : Core.Convert.t_From #t_ErrorCode #(Sandwich_proto.Errors.t_HandshakeError & v_S)
+    : Core.Convert.t_From t_ErrorCode (Sandwich_proto.Errors.t_HandshakeError & v_S)
 
 /// Instantiates an [`ErrorCode`] from an error enum and a string.
 [@@ FStar.Tactics.Typeclasses.tcinstance]
-val impl_120:Core.Convert.t_From #t_ErrorCode #(Sandwich_proto.Errors.t_HandshakeError & string)
+val impl_120:Core.Convert.t_From t_ErrorCode (Sandwich_proto.Errors.t_HandshakeError & string)
 
 /// Instantiates an [`ErrorCode`] from an error enum and a [`String`].
 [@@ FStar.Tactics.Typeclasses.tcinstance]
-val impl_121:Core.Convert.t_From #t_ErrorCode
-  #(Sandwich_proto.Errors.t_HandshakeError & Alloc.String.t_String)
+val impl_121:Core.Convert.t_From t_ErrorCode
+  (Sandwich_proto.Errors.t_HandshakeError & Alloc.String.t_String)
 
 /// Implements `[From<sandwich_proto::ErrorEnum>]` for [`ErrorCode`].
 [@@ FStar.Tactics.Typeclasses.tcinstance]
-val impl_127:Core.Convert.t_From #t_ErrorCode #Sandwich_proto.Errors.t_TunnelError
+val impl_127:Core.Convert.t_From t_ErrorCode Sandwich_proto.Errors.t_TunnelError
 
 /// Instantiates an [`ErrorCode`] from an error enum and a string.
 [@@ FStar.Tactics.Typeclasses.tcinstance]
 val impl_128 (#v_S: Type0) {| i1: Core.Convert.t_AsRef v_S string |}
-    : Core.Convert.t_From #t_ErrorCode #(Sandwich_proto.Errors.t_TunnelError & v_S)
+    : Core.Convert.t_From t_ErrorCode (Sandwich_proto.Errors.t_TunnelError & v_S)
 
 /// Instantiates an [`ErrorCode`] from an error enum and a string.
 [@@ FStar.Tactics.Typeclasses.tcinstance]
-val impl_129:Core.Convert.t_From #t_ErrorCode #(Sandwich_proto.Errors.t_TunnelError & string)
+val impl_129:Core.Convert.t_From t_ErrorCode (Sandwich_proto.Errors.t_TunnelError & string)
 
 /// Instantiates an [`ErrorCode`] from an error enum and a [`String`].
 [@@ FStar.Tactics.Typeclasses.tcinstance]
-val impl_130:Core.Convert.t_From #t_ErrorCode
-  #(Sandwich_proto.Errors.t_TunnelError & Alloc.String.t_String)
+val impl_130:Core.Convert.t_From t_ErrorCode
+  (Sandwich_proto.Errors.t_TunnelError & Alloc.String.t_String)
 
 /// Implements [`TryFrom`] for [`ProtoBasedErrorCode`].
 [@@ FStar.Tactics.Typeclasses.tcinstance]
-val impl_137:Core.Convert.t_TryFrom #t_ProtoBasedErrorCode #(i32 & i32)
+val impl_137:Core.Convert.t_TryFrom t_ProtoBasedErrorCode (i32 & i32)
 
 /// Implements [`TryFrom`] for [`ErrorCode`].
 [@@ FStar.Tactics.Typeclasses.tcinstance]
-val impl_138:Core.Convert.t_TryFrom #t_ErrorCode #(i32 & i32)
+val impl_138:Core.Convert.t_TryFrom t_ErrorCode (i32 & i32)
