proofs/fstar/extraction/Sandwich.Error.fsti
@@ -20,7 +20,7 @@ val impl
       (#v_ErrorEnum: Type0)
       {| i1: Sandwich.Error.Code.t_AllowedProtoBasedErrorCodeEnum v_ErrorEnum |}
       {| i2: Core.Convert.t_From Sandwich.Error.Code.t_ErrorCode v_ErrorEnum |}
-    : Core.Convert.t_From #t_Error #v_ErrorEnum
+    : Core.Convert.t_From t_Error v_ErrorEnum
 
 /// Instantiates an [`Error`] from an enum value and a string.
 [@@ FStar.Tactics.Typeclasses.tcinstance]
@@ -29,7 +29,7 @@ val impl_1
       {| i2: Sandwich.Error.Code.t_AllowedProtoBasedErrorCodeEnum v_ErrorEnum |}
       {| i3: Core.Convert.t_AsRef v_S string |}
       {| i4: Core.Convert.t_From Sandwich.Error.Code.t_ErrorCode (v_ErrorEnum & v_S) |}
-    : Core.Convert.t_From #t_Error #(v_ErrorEnum & v_S)
+    : Core.Convert.t_From t_Error (v_ErrorEnum & v_S)
 
 /// Instantiates an [`Error`] from an enum value and a string.
 [@@ FStar.Tactics.Typeclasses.tcinstance]
@@ -37,7 +37,7 @@ val impl_2
       (#v_ErrorEnum: Type0)
       {| i1: Sandwich.Error.Code.t_AllowedProtoBasedErrorCodeEnum v_ErrorEnum |}
       {| i2: Core.Convert.t_From Sandwich.Error.Code.t_ErrorCode (v_ErrorEnum & string) |}
-    : Core.Convert.t_From #t_Error #(v_ErrorEnum & string)
+    : Core.Convert.t_From t_Error (v_ErrorEnum & string)
 
 /// Instantiates an [`Error`] from an enum value and a string.
 [@@ FStar.Tactics.Typeclasses.tcinstance]
@@ -47,41 +47,41 @@ val impl_3
       {| i2:
           Core.Convert.t_From Sandwich.Error.Code.t_ErrorCode (v_ErrorEnum & Alloc.String.t_String)
         |}
-    : Core.Convert.t_From #t_Error #(v_ErrorEnum & Alloc.String.t_String)
+    : Core.Convert.t_From t_Error (v_ErrorEnum & Alloc.String.t_String)
 
 /// Instantiates an [`Error`] from an [`ProtoBasedErrorCode`].
 [@@ FStar.Tactics.Typeclasses.tcinstance]
-val impl_4:Core.Convert.t_From #t_Error #Sandwich.Error.Code.t_ProtoBasedErrorCode
+val impl_4:Core.Convert.t_From t_Error Sandwich.Error.Code.t_ProtoBasedErrorCode
 
 /// Instantiates an [`Error`] from an enum value and a string.
 [@@ FStar.Tactics.Typeclasses.tcinstance]
 val impl_5 (#v_S: Type0) {| i1: Core.Convert.t_AsRef v_S string |}
-    : Core.Convert.t_From #t_Error #(Sandwich.Error.Code.t_ProtoBasedErrorCode & v_S)
+    : Core.Convert.t_From t_Error (Sandwich.Error.Code.t_ProtoBasedErrorCode & v_S)
 
 /// Instantiates an [`Error`] from an enum value and a string.
 [@@ FStar.Tactics.Typeclasses.tcinstance]
-val impl_6:Core.Convert.t_From #t_Error #(Sandwich.Error.Code.t_ProtoBasedErrorCode & string)
+val impl_6:Core.Convert.t_From t_Error (Sandwich.Error.Code.t_ProtoBasedErrorCode & string)
 
 /// Instantiates an [`Error`] from an enum value and a string.
 [@@ FStar.Tactics.Typeclasses.tcinstance]
-val impl_7:Core.Convert.t_From #t_Error
-  #(Sandwich.Error.Code.t_ProtoBasedErrorCode & Alloc.String.t_String)
+val impl_7:Core.Convert.t_From t_Error
+  (Sandwich.Error.Code.t_ProtoBasedErrorCode & Alloc.String.t_String)
 
 /// Instantiates an [`Error`] from an [`ErrorCode`].
 [@@ FStar.Tactics.Typeclasses.tcinstance]
-val impl_8:Core.Convert.t_From #t_Error #Sandwich.Error.Code.t_ErrorCode
+val impl_8:Core.Convert.t_From t_Error Sandwich.Error.Code.t_ErrorCode
 
 /// Implements [`std::fmt::Display`] for [`Error`].
 [@@ FStar.Tactics.Typeclasses.tcinstance]
-val impl_18:Core.Fmt.t_Display #t_Error
+val impl_18:Core.Fmt.t_Display t_Error
 
 /// Implements [`std::fmt::Debug`] for [`Error`].
 [@@ FStar.Tactics.Typeclasses.tcinstance]
-val impl_19:Core.Fmt.t_Debug #t_Error
+val impl_19:Core.Fmt.t_Debug t_Error
 
 /// Implements [`std::error::Error`] for [`Error`].
 [@@ FStar.Tactics.Typeclasses.tcinstance]
-val impl_20:Core.Error.t_Error #t_Error
+val impl_20:Core.Error.t_Error t_Error
 
 /// Appends an [`Error`] into the chain, using the `>>` operator.
 /// The `>>` operator is used to easily build a chain of error:
@@ -103,7 +103,7 @@ val impl_9
       (#v_ErrorEnum: Type0)
       {| i1: Sandwich.Error.Code.t_AllowedProtoBasedErrorCodeEnum v_ErrorEnum |}
       {| i2: Core.Convert.t_From Sandwich.Error.Code.t_ErrorCode v_ErrorEnum |}
-    : Core.Ops.Bit.t_Shr #t_Error #v_ErrorEnum
+    : Core.Ops.Bit.t_Shr t_Error v_ErrorEnum
 
 /// Appends an [`Error`] into the chain, using the `>>` operator and a string.
 [@@ FStar.Tactics.Typeclasses.tcinstance]
@@ -112,7 +112,7 @@ val impl_10
       {| i2: Sandwich.Error.Code.t_AllowedProtoBasedErrorCodeEnum v_ErrorEnum |}
       {| i3: Core.Convert.t_From Sandwich.Error.Code.t_ErrorCode (v_ErrorEnum & v_S) |}
       {| i4: Core.Convert.t_AsRef v_S string |}
-    : Core.Ops.Bit.t_Shr #t_Error #(v_ErrorEnum & v_S)
+    : Core.Ops.Bit.t_Shr t_Error (v_ErrorEnum & v_S)
 
 /// Appends an [`Error`] into the chain, using the `>>` operator and a string.
 [@@ FStar.Tactics.Typeclasses.tcinstance]
@@ -120,7 +120,7 @@ val impl_11
       (#v_ErrorEnum: Type0)
       {| i1: Sandwich.Error.Code.t_AllowedProtoBasedErrorCodeEnum v_ErrorEnum |}
       {| i2: Core.Convert.t_From Sandwich.Error.Code.t_ErrorCode (v_ErrorEnum & string) |}
-    : Core.Ops.Bit.t_Shr #t_Error #(v_ErrorEnum & string)
+    : Core.Ops.Bit.t_Shr t_Error (v_ErrorEnum & string)
 
 /// Appends an [`Error`] into the chain, using the `>>` operator and a string.
 [@@ FStar.Tactics.Typeclasses.tcinstance]
@@ -130,31 +130,31 @@ val impl_12
       {| i2:
           Core.Convert.t_From Sandwich.Error.Code.t_ErrorCode (v_ErrorEnum & Alloc.String.t_String)
         |}
-    : Core.Ops.Bit.t_Shr #t_Error #(v_ErrorEnum & Alloc.String.t_String)
+    : Core.Ops.Bit.t_Shr t_Error (v_ErrorEnum & Alloc.String.t_String)
 
 /// Appends an [`Error`] into the chain, using the `>>` operator.
 [@@ FStar.Tactics.Typeclasses.tcinstance]
-val impl_13:Core.Ops.Bit.t_Shr #t_Error #Sandwich.Error.Code.t_ProtoBasedErrorCode
+val impl_13:Core.Ops.Bit.t_Shr t_Error Sandwich.Error.Code.t_ProtoBasedErrorCode
 
 /// Appends an [`Error`] into the chain, using the `>>` operator and a string.
 [@@ FStar.Tactics.Typeclasses.tcinstance]
 val impl_14 (#v_S: Type0) {| i1: Core.Convert.t_AsRef v_S string |}
-    : Core.Ops.Bit.t_Shr #t_Error #(Sandwich.Error.Code.t_ProtoBasedErrorCode & v_S)
+    : Core.Ops.Bit.t_Shr t_Error (Sandwich.Error.Code.t_ProtoBasedErrorCode & v_S)
 
 /// Appends an [`Error`] into the chain, using the `>>` operator and a string.
 [@@ FStar.Tactics.Typeclasses.tcinstance]
-val impl_15:Core.Ops.Bit.t_Shr #t_Error #(Sandwich.Error.Code.t_ProtoBasedErrorCode & string)
+val impl_15:Core.Ops.Bit.t_Shr t_Error (Sandwich.Error.Code.t_ProtoBasedErrorCode & string)
 
 /// Appends an [`Error`] into the chain, using the `>>` operator.
 [@@ FStar.Tactics.Typeclasses.tcinstance]
-val impl_16:Core.Ops.Bit.t_Shr #t_Error
-  #(Sandwich.Error.Code.t_ProtoBasedErrorCode & Alloc.String.t_String)
+val impl_16:Core.Ops.Bit.t_Shr t_Error
+  (Sandwich.Error.Code.t_ProtoBasedErrorCode & Alloc.String.t_String)
 
 /// Appends an [`Error`] into the chain, using the `>>` operator.
 [@@ FStar.Tactics.Typeclasses.tcinstance]
-val impl_17:Core.Ops.Bit.t_Shr #t_Error #Sandwich.Error.Code.t_ErrorCode
+val impl_17:Core.Ops.Bit.t_Shr t_Error Sandwich.Error.Code.t_ErrorCode
 
 /// Implements operator>> between two [`ErrorCode`] to produce
 /// an [`Error`].
 [@@ FStar.Tactics.Typeclasses.tcinstance]
-val impl_22:Core.Ops.Bit.t_Shr #Sandwich.Error.Code.t_ErrorCode #Sandwich.Error.Code.t_ErrorCode
+val impl_22:Core.Ops.Bit.t_Shr Sandwich.Error.Code.t_ErrorCode Sandwich.Error.Code.t_ErrorCode
