proofs/fstar/extraction/Sandwich.Support.Data_source.fst
@@ -3,23 +3,6 @@ module Sandwich.Support.Data_source
 open Core
 open FStar.Mul
 
-/// A source of data.
-/// Source of the material is either from the local filesystem (`Fs`), from
-/// an inline slice of bytes (`Bytes`) or from a inline string (`String`).
-/// The content is borrowed, unless is it explicitly mandated to own it.
-type t_DataSource =
-  | DataSource_Fs : Alloc.Vec.t_Vec u8 Alloc.Alloc.t_Global -> t_DataSource
-  | DataSource_Bytes : Alloc.Borrow.t_Cow (t_Slice u8) -> t_DataSource
-  | DataSource_String : Alloc.Borrow.t_Cow string -> t_DataSource
-
-/// Returns the data holds by the [`DataSource`] as a slice of bytes.
-[@@ FStar.Tactics.Typeclasses.tcinstance]
-val impl_1:Core.Convert.t_AsRef t_DataSource (t_Slice u8)
-
-/// Implements [`std::fmt::Debug`] for [`DataSource`].
-[@@ FStar.Tactics.Typeclasses.tcinstance]
-val impl_2:Core.Fmt.t_Debug t_DataSource
-
 (* item error backend: (reject_RawOrMutPointer) ExplicitRejection { reason: "a node of kind [Raw_pointer] have been found in the AST" }
 Last available AST for this item:
 
@@ -41,13 +24,3 @@ Last AST:
   kind = Concrete_ident.Kind.Value }) */
 const _: () = ();
  *)
-
-/// Instantiates a [`DataSource`] from a protobuf `DataSource` message.
-/// # Errors
-/// If the protobuf `DataSource` message provides a filename, and the file
-/// couldn't be found or read from the local filesystem, then
-/// `DataSourceError::DATASOURCEERROR_NOT_FOUND` is returned.
-/// If the protobuf `DataSource` message doesn't provide any source type,
-/// then `DataSourceError::DATASOURCEERROR_INVALID_CASE` is returned.
-[@@ FStar.Tactics.Typeclasses.tcinstance]
-val impl:Core.Convert.t_TryFrom t_DataSource Sandwich_api_proto.Data_source.t_DataSource
